today's lesson: emacs auto-save is *f******** unreliable.
also: don't forget to press save.
just lost three days of work due to emacs/coq crashing... :)

theories/L/Complexity/Cook/GenNP_GenNPInter_Basics.v
@@ -125,25 +125,6 @@ Module basics (sig : TMSig).
   Notation negative := L. 
   Notation neutral := N. 
 
-
-  (* Inductive polarity := positive | negative | neutral.  *)
-  (* Hint Constructors polarity.  *)
-
-  (* Instance polarity_eqTypeC : eq_dec polarity.  *)
-  (* Proof.  *)
-  (*   unfold dec. decide equality.  *)
-  (* Qed.  *)
-
-  (* Lemma polarity_Enum_Ok x : BasicDefinitions.count [positive; negative; neutral] x = 1.  *)
-  (* Proof.  *)
-  (*   simpl; dec; destruct x; congruence.  *)
-  (* Qed.  *)
-
-  (* Instance polarity_finTypeC : finTypeC (EqType polarity).  *)
-  (* Proof.  *)
-  (*   econstructor. apply polarity_Enum_Ok.  *)
-  (* Defined.  *)
-
   Implicit Type σ : Sigma. 
 
   Notation "'↓' σ" := ((negative, σ)) (at level 30). 
@@ -160,40 +141,20 @@ Module basics (sig : TMSig).
 
   Notation "$" := (inl delimC). 
 
-  Notation polSigma := ((polarity * Sigma)%type).
-  Notation tapeSigma' := (option polSigma). 
-  Notation tapeSigma := (sum delim tapeSigma').
-
   Notation stateSigma := (option Sigma). 
-
+  Notation polSigma := ((polarity * stateSigma)%type).
+  Notation tapeSigma := (sum delim polSigma).
   Notation States := ((states * stateSigma)%type). 
-
   Notation Gamma := ((States + tapeSigma)%type). 
  
 
   Implicit Type (γ : Gamma).
   Implicit Type (q : states).
-  Implicit Type (m : tapeSigma).
+  Implicit Type (m : stateSigma).
   Implicit Type (p : polarity).
 
-  (* Definition inra := @inr States tapeSigma. *)
-  (* Coercion inra : tapeSigma >-> Gamma. *)
 
   Notation "'|_|'" := (None). 
-
-  (*move tape element from state to tape cell, adding a polarity*)
-  Definition withPolaritySigma p σ : tapeSigma := inr(Some (p, σ)). 
-  Definition withPolarity p (σ: stateSigma) : tapeSigma := match σ with |_| => inr |_| | Some σ => (withPolaritySigma p σ)  end.
-
-  (*move from tape cell to state cell *)
-  Definition removePolarity (σ : tapeSigma') : stateSigma := match σ with |_| => |_| | Some (p, σ) => Some σ end.
-
-  Notation "p ! a" := (withPolarity p a) (at level 5). 
-  Notation "p !! a" := (withPolaritySigma p a) (at level 5). 
-
-  Hint Unfold withPolarity. 
-
-  Definition setPolarity p (σ : polSigma) : polSigma := match σ with (_, σ) => (p, σ) end. 
 
   (*flip the polarity of a symbol *)
   Definition polarityFlip p := match p with negative => positive | positive => negative | neutral => neutral end. 
@@ -208,48 +169,37 @@ Module basics (sig : TMSig).
 
   Smpl Add (apply polarityFlipSigma_involution) : involution. 
 
-  Definition polarityFlipTapeSigma' (x : tapeSigma') : tapeSigma' := match x with |_| => |_| | Some σ => Some (polarityFlipSigma σ) end. 
-  Definition polarityFlipTapeSigma (x : tapeSigma) : tapeSigma := match x with inr a => inr (polarityFlipTapeSigma' a) | $ => $ end. 
+  Definition polarityFlipTapeSigma (x : tapeSigma) : tapeSigma := match x with inr a => inr (polarityFlipSigma a) | $ => $ end. 
   Definition polarityFlipGamma (x : Gamma) : Gamma := match x with inl s => inl s | inr x => inr (polarityFlipTapeSigma x) end.
 
   Notation "'~' x" := (polarityFlipGamma x). 
-  Notation "'#' x" := (polarityFlipTapeSigma' x) (at level 1). 
+  Notation "'!' x" := (polarityFlipSigma x) (at level 1). 
   Notation "'%' x" := (polarityFlipTapeSigma x) (at level 30). 
-
-  Lemma polarityFlipTapeSigma'_involution : involution polarityFlipTapeSigma'.
-  Proof. intros x. destruct x; [ | now cbn]. cbn. now rewrite polarityFlipSigma_involution. Qed. 
 
   Lemma polarityFlipTapeSigma_involution : involution polarityFlipTapeSigma.
   Proof.
-    intros x. destruct x; [ destruct d; now cbn | ]. cbn; now rewrite polarityFlipTapeSigma'_involution.
+    intros x. destruct x; [ destruct d; now cbn | ]. destruct p; cbn. now rewrite polarityFlip_involution. 
   Qed. 
   Lemma polarityFlipGamma_involution : involution polarityFlipGamma. 
   Proof. 
     intros x. destruct x; [now cbn | ]. cbn. now rewrite polarityFlipTapeSigma_involution.  
   Qed. 
 
-  Smpl Add (apply polarityFlipTapeSigma'_involution) : involution.
   Smpl Add (apply polarityFlipTapeSigma_involution) : involution.
   Smpl Add (apply polarityFlipGamma_involution) : involution.
   
-  Lemma polarityFlipSigmaInv1 e p σ : polarityFlipSigma e = (p, σ) -> e = (polarityFlip p, σ). 
+  Lemma polarityFlipSigmaInv1 e p m : polarityFlipSigma e = (p, m) -> e = (polarityFlip p, m). 
   Proof. 
     unfold polarityFlipSigma. destruct e as [p' e]. intros. inv H. specialize (polarityFlip_involution p'). congruence. 
   Qed. 
 
-  Lemma polarityFlipTapeSigma'Inv1 e p σ : polarityFlipTapeSigma' e = (Some (p, σ)) -> e = (Some (polarityFlip p, σ)). 
-  Proof.
-    intros; destruct e; cbn in H; [ | congruence]. inv H.
-    now apply polarityFlipSigmaInv1 in H1.  
-  Qed. 
-
-  Lemma polarityFlipTapeSigmaInv1 e p σ : polarityFlipTapeSigma e = inr (Some (p, σ)) -> e = inr (Some (polarityFlip p, σ)). 
+  Lemma polarityFlipTapeSigmaInv1 e p m : polarityFlipTapeSigma e = inr (p, m) -> e = inr (polarityFlip p, m). 
   Proof.
     intros. destruct e; cbn in H; [destruct d; congruence | ].
-    inv H. now apply polarityFlipTapeSigma'Inv1 in H1. 
+    inv H. now apply polarityFlipSigmaInv1 in H1. 
   Qed. 
 
-  Lemma polarityFlipGammaInv1 e p σ : polarityFlipGamma e = inr (inr (Some (p, σ))) -> e = inr (inr (Some (polarityFlip p, σ))). 
+  Lemma polarityFlipGammaInv1 e p m : polarityFlipGamma e = inr (inr (p, m)) -> e = inr (inr (polarityFlip p, m)). 
   Proof. 
     intros. destruct e; cbn in H; [ congruence | ]. 
     inv H. now apply polarityFlipTapeSigmaInv1 in H1.
@@ -271,40 +221,34 @@ Module basics (sig : TMSig).
 
 
   (** *representation of tapes *)
-  Definition stape := list Sigma. 
+  Notation stape := (list Sigma). 
   Implicit Type (u v : stape). 
 
-  Definition halftape := list Gamma.
+  Notation halftape := (list Gamma).
   Implicit Type (h : halftape). 
 
 
   (*a string consisting of k blanks*)
-  Fixpoint E k : halftape := match k with 0 => [inr $] | S k => inr (inr |_|) :: E k end. 
-
-  Lemma E_length (v  : nat) : |(E v)| = S v. 
+  Fixpoint E p k : halftape := match k with 0 => [inr $] | S k => inr (inr (p, |_|)) :: E p k end. 
+  Lemma E_length p n: |(E p n)| = S n. 
   Proof. 
-    induction v; cbn.
+    induction n; cbn.
     - reflexivity.  
-    - rewrite <- IHv at 1. reflexivity.  (*slightly hacky because of typeclass inference *)
+    - rewrite <- IHn at 1. reflexivity.  (*slightly hacky because of typeclass inference *)
   Qed. 
 
-  Lemma E_w_step w : E (wo + w) = (inr (inr |_|)) :: E (wo + w -1).
+  Lemma E_w_step p w : E p (wo + w) = (inr (inr (p, |_|))) :: E p (wo + w -1).
   Proof.
     remember (w + wo). destruct n. 
     + unfold wo in Heqn; lia. 
     + now cbn. 
   Qed. 
 
-  Lemma E_w_head w : E (wo + w) = (inr (inr |_|)) :: (inr(inr |_|)) :: E w. 
-  Proof. 
-    remember (w + wo); unfold wo in Heqn. destruct n; [ lia | destruct n; [lia | ]]. now cbn. 
-  Qed. 
-
-  Lemma E_polarityFlip n : map polarityFlipGamma (E n) = E n. 
+  Lemma E_polarityFlip p n : map polarityFlipGamma (E p n) = E (polarityFlip p) n. 
   Proof. induction n; cbn; now f_equal. Qed. 
 
-  Definition mapPolarity p u : list Gamma := map (fun e => inr (withPolaritySigma p e)) u.
-  Definition reprTape' w u h p:= length h = S wo + w /\ length u <= w /\ h = (mapPolarity p u) ++ E ( wo + w - (|u|)). 
+  Definition mapPolarity p u : list Gamma := map (fun e => inr (inr (p, Some e))) u.
+  Definition reprTape' w u h p:= length h = S wo + w /\ length u <= w /\ h = (mapPolarity p u) ++ E p ( wo + w - (|u|)). 
 
   Definition reprTape := reprTape' z'. 
 
@@ -313,7 +257,7 @@ Module basics (sig : TMSig).
 
   Notation "u '≃t(' p ',' w ')' h" := (reprTape' w u h p) (at level 80). 
 
-  Lemma niltape_repr : forall w p, [] ≃t(p, w) (E (wo + w)) /\ forall a, [] ≃t(p, w) a -> a = E (wo + w). 
+  Lemma niltape_repr : forall w p, [] ≃t(p, w) (E p (wo + w)) /\ forall a, [] ≃t(p, w) a -> a = E p (wo + w). 
   Proof.
     intros. repeat split.
     - apply E_length. 
@@ -334,35 +278,14 @@ Module basics (sig : TMSig).
   Qed. 
 
   (** *representation of configurations *)
-  Definition strconfig := list Gamma.
+  Notation strconfig := (list Gamma).
   Implicit Type (s x : strconfig).
 
   Definition embedState (q : states) (m : stateSigma) : Gamma := inl (q, m). 
   Definition reprConfig' c ls qm rs := match c with (q, tape) => exists p, qm = embedState q (current tape) /\ reprTape (left tape) ls p /\ reprTape (right tape) rs p end. 
   Definition reprConfig c (s : list Gamma) := exists ls qm rs, s = rev ls ++ [qm] ++ rs /\ reprConfig' c ls qm rs. 
-  (* Definition reprConfig c (s : list Gamma) := match c with (q, tape) => match tape with *)
-  (*                                               | niltape _ => s = rev (E z) ++ [embedState q |_|] ++ E z *)
-  (*                                               | leftof r rs => exists h, (r :: rs) ≃t h /\ s = rev (E z) ++ [embedState q |_|] ++ h *)
-  (*                                               | rightof r rs => exists h, (r :: rs) ≃t h /\ s = rev h ++ [embedState q |_|] ++ E z *)
-  (*                                               | midtape ls m rs => exists p h1 h2, ls ≃t(p) h1 /\ rs ≃t(p) h2 /\ s = rev h1 ++ [embedState q (Some m)] ++ h2 *)
-  (*                                              end end.  *)
 
   Notation "c '≃c' '(' ls ',' q ',' rs ')'" := (reprConfig' c ls q rs) (at level 80). 
   Notation "c '≃c' s" := (reprConfig c s) (at level 80). 
-
-  Definition getState s : option States := match nth_error s (S z) with None => None | Some q => match q with inl q => Some q | inr _ => None end end.  
-  (*tape positions are one-based *)
-  Definition getLeft s n : option tapeSigma := match nth_error s (S z - n) with None => None |  Some q => match q with inr q => Some q | inl _ => None end end.
-  Definition getRight s n : option tapeSigma := match nth_error s (S z + n) with None => None | Some q => match q with inr q => Some q | inl _ => None end end. 
-
-  Lemma getState_Some q tape s : (q, tape) ≃c s -> getState s = Some (q, current tape). 
-  Proof. 
-    intros. destruct H as (ls & qm & rs & -> & H).
-    destruct H as (p & -> & H1 & H2). 
-    unfold getState. destruct H1. rewrite nth_error_app2. 
-    all: rewrite rev_length, H; unfold z, z'.
-    2: lia. 
-    cbn. rewrite Nat.sub_diag. now cbn.
-  Qed. 
 
 End basics. 
